theories/Pair.ec
@@ -4,6 +4,19 @@ op fst (p:'a * 'b): 'a =
 op snd (p:'a * 'b): 'b = 
   let (a,b) = p in b.
 
+lemma nosmt pw_eq (x x':'a) (y y':'b):
+  x = x' => y = y' => (x,y) = (x',y')
+by [].
+
+lemma nosmt pairS (x:'a * 'b): x = (fst x,snd x)
+by [].
+
+lemma nosmt fst_pair (y:'b) (x:'a): fst (x,y) = x
+by trivial.
+
+lemma nosmt snd_pair (x:'a) (y:'b): snd (x,y) = y
+by trivial.
+
 require import Real.
 require import Distr.
 
